

List of topics in this lecture

- A mathematical derivation of Smoluchowski-Kramers approximation
- Scaling of X , Y and $F(X, t)$
- The method of solvability condition

Recap

Smoluchowski-Kramers approximation

Langevin equation for a small particle in water

$$dX = Y dt$$

$$mdY = -bY dt + F(X, t)dt + \sqrt{2k_b T b} dW$$

where X : position; Y : velocity;

a : radius of the particle;

$m = 4\pi/3 a^3 = O(a^3)$: mass of the particle

$b = 6\pi \eta a = O(a)$: drag coefficient of the particle

Time scale of inertia and thermal excitation: $t_0 = m/b = O(a^2)$

S-K approximation:

For $t_{\text{scale}} \gg t \gg t_0$, $X(t)$ satisfies

$$X(t) - X(0) = \underbrace{\frac{F_0}{b}t}_{\text{Term III}} + \underbrace{t_0 \left(Y(0) - \frac{F_0}{b} \right)}_{\text{Term I}} + \underbrace{N \left(0, (\gamma t_0)^2 t_0 \left(\frac{t}{t_0} \right) \right)}_{\text{Term II}} + \text{T.S.T.} \quad (\text{SK0})$$

where t_{scale} is the time scale of physical evolution. We neglect Term I, and keep Term II and Term III. On a “coarse” grid, $X(t)$ is governed by

$$dX = \frac{F(X, t)}{b} dt + \sqrt{2D} dW$$

A mathematical derivation of Smoluchowski-Kramers approximation

Let $\varepsilon \equiv \sqrt{t_0 / t_{\text{scale}}} = O(a/R)$ be a small parameter.

Here t_{scale} is the time scale of physical evolution and R is a size scale whose time scale of inertia is t_{scale} . We assume that **the time is measured in units of t_{scale}** , and the particle position/size is measured in units of R . We write $O(a/R)$ simply as $O(a)$.

Scaling of position X

The over-damped Langevin equation for X is

$$dX = \frac{F(X,t)}{b} dt + \sqrt{2D} dW, \quad D = O(a^{-1}) = O(\varepsilon^{-1})$$

This equation is not free of ε . When $F = 0$ and $t = O(1)$, we have

$$X(1) - X(0) \sim \sqrt{2D} = O(\varepsilon^{-1/2})$$

We select a scaling for X to make it $O(1)$.

$$\hat{X} = \sqrt{\varepsilon} X \Rightarrow \hat{X}(1) - \hat{X}(0) = O(1)$$

The over-damped Langevin equation after scaling X

We consider the case where for $t = O(1)$, the effect of external driving force is comparable to that of the diffusion

$$\frac{F(X,t)}{b} = O(\sqrt{D}) = O(\varepsilon^{-1/2}), \quad b = O(a) = O(\varepsilon)$$

$$\Rightarrow F(X,t) = O(\sqrt{\varepsilon})$$

After scaling X , we have

$$\sqrt{\varepsilon} dX = \sqrt{\varepsilon} \frac{F(X,t)}{b} dt + \sqrt{\varepsilon} \sqrt{2D} dW$$

$$\Rightarrow \boxed{d\hat{X} = f(\hat{X}, t) dt + \sqrt{2D_0} dW}$$

where

$$D_0 \equiv \varepsilon D = O(1), \quad f(\hat{X}, t) \equiv \sqrt{\varepsilon} \frac{F(X,t)}{b} = O(1)$$

Note: after scaling X , the over-damped Langevin equation is free of ε .

Scaling of velocity Y

We scale Y separately from the scaling of X . Here Y is the instantaneous velocity, dominated by thermal excitations, much larger than $X(1) - X(0)$.

When $F = 0$, the equipartition of energy gives us

$$\sqrt{E(Y^2)} = \sqrt{\frac{k_B T}{m}} = O(\epsilon^{-3/2}), \quad m = O(a^3) = O(\epsilon^3)$$

We select a scaling for Y to make it $O(1)$

$$\hat{Y} = \epsilon^{3/2} Y \Rightarrow \sqrt{E(\hat{Y}^2)} = O(1)$$

The FULL Langevin equation after scaling of Y

$$m dY = -bY dt + F(X, t)dt + b\sqrt{2D} dW$$

$$\Rightarrow \frac{m}{b} dY = -Y dt + \frac{F(X, t)}{b} dt + \sqrt{2D} dW$$

$$\Rightarrow \epsilon^2 (\epsilon^{-3/2} d\hat{Y}) = -(\epsilon^{-3/2} \hat{Y}) dt + \epsilon^{-1/2} f(\hat{X}, t) dt + \sqrt{2(\epsilon^{-1} D_0)} dW$$

$$\Rightarrow \epsilon^{1/2} d\hat{Y} = -\epsilon^{-3/2} \hat{Y} dt + \epsilon^{-1/2} f(\hat{X}, t) dt + \epsilon^{-1/2} \sqrt{2D_0} dW$$

$$\Rightarrow \boxed{d\hat{Y} = \frac{-1}{\epsilon^2} \hat{Y} dt + \frac{1}{\epsilon} f(\hat{X}, t) dt + \frac{1}{\epsilon} \sqrt{2D_0} dW}$$

Since X and Y are scaled separately, after scaling they are related by

$$dX = Y dt \Rightarrow d(\epsilon^{1/2} X) = \epsilon^{-1} (\epsilon^{3/2} Y) dt \Rightarrow d\hat{X} = \epsilon^{-1} \hat{Y} dt$$

Notation:

After scaling, we recycle the simple notation of (X, Y, t) to write out the starting SDE and the end SDE of the S-K approximation.

The starting SDE of S-K approximation

$$\begin{aligned} dX &= \frac{1}{\epsilon} Y dt \\ dY &= \frac{-1}{\epsilon^2} Y dt + \frac{1}{\epsilon} f(X, t) dt + \frac{1}{\epsilon} \sqrt{2D_0} dW \end{aligned} \tag{S-1}$$

The end SDE of S-K approximation

$$dX = f(X, t) dt + \sqrt{2D_0} dW \tag{S-2}$$

Backward equation for the starting SDE

For the starting SDE (S-1), we consider function

$$u(x, y, t) \equiv \Pr \left\{ X \text{ having crossed } x_b \text{ by time } t \mid X(0) = x, Y(0) = y \right\}$$

We derive the governing equation of $u(x, y, t)$. For dt small enough, we have

$$u(x, y, t) = E(u(x + dX, y + dY, t - dt)) + o(dt) \quad (E-1)$$

Note that in the SDE, $\varepsilon = \text{fixed}$. As $dt \rightarrow 0$, we have $dX = O(dt)$ and $dY = O(\sqrt{dt})$.

Specifically we have the moments of dX and dY from the SDE.

$$(dX | X(0) = x, Y(0) = y) = \frac{y}{\varepsilon} dt \quad \text{not a random variable}$$

$$E(dY | X(0) = x, Y(0) = y) = \left(\frac{-1}{\varepsilon^2} y + \frac{1}{\varepsilon} f(x, t) \right) dt$$

$$E((dY)^2 | X(0) = x, Y(0) = y) = \frac{1}{\varepsilon^2} 2D_0 dt + o(dt)$$

$$E((dY)^n | X(0) = x, Y(0) = y) = o(dt) \quad \text{for } n \geq 3$$

We expand (E-1)

$$\begin{aligned} u(x, y, t) &= E(u(x + dX, y + dY, t - dt)) + o(dt) \\ &= E \left(u(x, y, t) + u_x dX + u_y dY + \frac{1}{2} u_{yy} (dY)^2 - u_t dt \right) + o(dt) \\ &= u + u_x \frac{y}{\varepsilon} dt + u_y \left(\frac{-1}{\varepsilon^2} y + \frac{1}{\varepsilon} f(x, t) \right) dt + \frac{1}{2} u_{yy} \frac{1}{\varepsilon^2} 2D_0 dt - u_t dt + o(dt) \\ &\quad \dots \end{aligned}$$

The governing equation for $u(x, y, t)$ is the backward equation of (S-1).

$$\varepsilon^2 u_t = -y u_y + D_0 u_{yy} + \varepsilon (y u_x + f(x, t) u_y) \quad (BE-1)$$

Backward equation for the end SDE

For the end SDE (S-2), we consider function

$$w(x, t) \equiv \Pr \{ X \text{ having crossed } x_B \text{ by time } t | X(0) = x \}$$

The governing equation for $w(x, t)$ is the backward equation of (S-2).

$$\frac{\partial w}{\partial t} = D_0 \frac{\partial^2 w}{\partial x^2} + f(x, t) \frac{\partial w}{\partial x} \quad (BE-2)$$

Convergence of $u(x, y, t)$ to $w(x, t)$

For backward equation (BE-1), we seek solutions of the form

$$u(x, y, t) = u_0(x, y, t) + \varepsilon u_1(x, y, t) + \varepsilon^2 u_2(x, y, t) + \dots$$

We substitute the expansion into (BE-1) and keep terms up to $O(\varepsilon^2)$.

$$\begin{aligned} \varepsilon^2 \frac{\partial u_0}{\partial t} &= -y \left(\frac{\partial u_0}{\partial y} + \varepsilon \frac{\partial u_1}{\partial y} + \varepsilon^2 \frac{\partial u_2}{\partial y} \right) + D_0 \left(\frac{\partial^2 u_0}{\partial y^2} + \varepsilon \frac{\partial^2 u_1}{\partial y^2} + \varepsilon^2 \frac{\partial^2 u_2}{\partial y^2} \right) \\ &\quad + \varepsilon \left(y \left(\frac{\partial u_0}{\partial x} + \varepsilon \frac{\partial u_1}{\partial x} \right) + f(x, t) \left(\frac{\partial u_0}{\partial y} + \varepsilon \frac{\partial u_1}{\partial y} \right) \right) + o(\varepsilon^2) \\ \implies 0 &= \underbrace{\left(-y \frac{\partial u_0}{\partial y} + D_0 \frac{\partial^2 u_0}{\partial y^2} \right)}_{O(1) \text{ terms}} + \underbrace{\varepsilon \left(-y \frac{\partial u_1}{\partial y} + D_0 \frac{\partial^2 u_1}{\partial y^2} + y \frac{\partial u_0}{\partial x} + f(x, t) \frac{\partial u_0}{\partial y} \right)}_{O(\varepsilon) \text{ terms}} \\ &\quad + \underbrace{\varepsilon^2 \left(-y \frac{\partial u_2}{\partial y} + D_0 \frac{\partial^2 u_2}{\partial y^2} + y \frac{\partial u_1}{\partial x} + f(x, t) \frac{\partial u_1}{\partial y} - \frac{\partial u_0}{\partial t} \right)}_{O(\varepsilon^2) \text{ terms}} + o(\varepsilon^2) \end{aligned}$$

Below, we show that

- $u_0(x, y, t) = u_0(x, t)$, independent of y .
- $u_0(x, t)$ satisfies backward equation (BE-2).

Step A: $u_0(x, y, t)$ is independent of y .

The balance of $O(1)$ terms gives the equation

$$-y \frac{\partial u_0}{\partial y} + D_0 \frac{\partial^2 u_0}{\partial y^2} = 0$$

Multiplying by the integrating factor yields

$$\begin{aligned} \exp\left(\frac{-y^2}{2D_0}\right) \left(\frac{-y}{D_0} \right) \frac{\partial u_0}{\partial y} + \exp\left(\frac{-y^2}{2D_0}\right) \frac{\partial^2 u_0}{\partial y^2} &= 0 \\ \implies \frac{\partial}{\partial y} \left[\exp\left(\frac{-y^2}{2D_0}\right) \frac{\partial u_0}{\partial y} \right] &= 0 \\ \implies \exp\left(\frac{-y^2}{2D_0}\right) \frac{\partial u_0}{\partial y} &= c_1(x, t) \text{ independent of } y \end{aligned}$$

$$\implies \frac{\partial u_0}{\partial y} = c_1(x, t) \exp\left(\frac{y^2}{2D_0}\right)$$

$$\implies u_0 = c_0(x, t) + c_1(x, t) \int_0^y \exp\left(\frac{z^2}{2D_0}\right) dz$$

Recall that $u(x, y, t)$ = probability.

$$\implies u(x, y, t) \text{ is bounded as } y \rightarrow \infty.$$

$$\implies u_0(x, y, t), \text{ as the leading term, is bounded as } y \rightarrow \infty$$

$$\implies c_1(x, t) = 0$$

$$\implies u_0 = c_0(x, t) \quad \text{independent of } y$$

Step B: $u_0(x, t)$ satisfies backward equation (BE-2)

Step B1: The balance of $O(\varepsilon)$ terms gives

$$-y \frac{\partial u_1}{\partial y} + D_0 \frac{\partial^2 u_1}{\partial y^2} + y \frac{\partial u_0}{\partial x} + f(x, t) \frac{\partial u_0}{\partial y} = 0$$

We write it as an equation for u_1 and multiply by the integrating factor

$$-y \frac{\partial u_1}{\partial y} + D_0 \frac{\partial^2 u_1}{\partial y^2} = -y \frac{\partial u_0}{\partial x}$$

$$\implies \exp\left(\frac{-y^2}{2D_0}\right) \left(\frac{-y}{D_0}\right) \frac{\partial u_1}{\partial y} + \exp\left(\frac{-y^2}{2D_0}\right) \frac{\partial^2 u_1}{\partial y^2} = \exp\left(\frac{-y^2}{2D_0}\right) \left(\frac{-y}{D_0}\right) \frac{\partial u_0}{\partial x}$$

$$\implies \frac{\partial}{\partial y} \left(\exp\left(\frac{-y^2}{2D_0}\right) \frac{\partial u_1}{\partial y} \right) = \frac{\partial}{\partial y} \left(\exp\left(\frac{-y^2}{2D_0}\right) \right) \frac{\partial u_0}{\partial x}$$

Noticing that $\partial u_0 / \partial x$ is independent of y and integrating in y , we get

$$\exp\left(\frac{-y^2}{2D_0}\right) \frac{\partial u_1}{\partial y} = \exp\left(\frac{-y^2}{2D_0}\right) \frac{\partial u_0}{\partial x} + c_3(x, t)$$

$$\implies \frac{\partial u_1}{\partial y} = \frac{\partial u_0}{\partial x} + c_3(x, t) \exp\left(\frac{y^2}{2D_0}\right)$$

$$\implies u_1 = y \frac{\partial u_0}{\partial x} + c_2(x, t) + c_3(x, t) \int_0^y \exp\left(\frac{z^2}{2D_0}\right) dz$$

u_1 is solvable without imposing any constraint on u_0 .

To find a constraint on u_0 , we need to examine $O(\varepsilon^2)$ terms.

Step B2: The balance of $O(\varepsilon^2)$ terms gives

$$\begin{aligned}
 & -y \frac{\partial u_2}{\partial y} + D_0 \frac{\partial^2 u_2}{\partial y^2} + y \frac{\partial u_1}{\partial x} + f(x, t) \frac{\partial u_1}{\partial y} - \frac{\partial u_0}{\partial t} = 0 \\
 \implies & -y \frac{\partial u_2}{\partial y} + D_0 \frac{\partial^2 u_2}{\partial y^2} = \frac{\partial u_0}{\partial t} - y \frac{\partial u_1}{\partial x} - f(x, t) \frac{\partial u_1}{\partial y} \\
 \implies & L_1[u_2] = \frac{\partial u_0}{\partial t} + L_2[u_1]
 \end{aligned}$$

where operators L_1 and L_2 are defined as

$$\begin{aligned}
 L_1[\cdot] & \equiv -y \frac{\partial \cdot}{\partial y} + D_0 \frac{\partial^2 \cdot}{\partial y^2} \\
 L_2[\cdot] & \equiv -y \frac{\partial \cdot}{\partial x} - f(x, t) \frac{\partial \cdot}{\partial y}
 \end{aligned}$$

Theorem (solvability condition)

Equation $L[u] = g$ is solvable if and only if $\langle g, v \rangle = 0$ for all v satisfying $L^*[v] = 0$
 (with $v(y) \rightarrow 0$ rapidly as $|y| \rightarrow \infty$)

A simple demonstration of the theorem:

Let A be an $m \times n$ matrix.

$Au = b$ is solvable if and only if $b \in \text{Col}(A)$

if and only if $\langle b, v \rangle = 0$ for all $v \in \text{Col}(A)^\perp = \text{Nul}(A^T)$.

if and only if $\langle b, v \rangle = 0$ for all v satisfying $A^T v = 0$.

Important note:

When operator L_1 is in variable y , we view $v(y)$ as a function of y and the inner-product $\langle g, v \rangle$ is an integral with respect to y .

Step B3: Solvability of $L_1[u_2] = \frac{\partial u_0}{\partial t} + L_2[u_1]$.

u_2 is solvable if and only if $\left\langle \frac{\partial u_0}{\partial t} + L_2[u_1], v \right\rangle = 0$ for all v satisfying $L_1^*[v] = 0$.

Step B4: Solution of $L_1^*[v] = 0$

$$L_1[\cdot] = -y \frac{\partial \cdot}{\partial y} + D_0 \frac{\partial^2 \cdot}{\partial y^2} \implies L_1^*[\cdot] = \frac{\partial(y \cdot)}{\partial y} + D_0 \frac{\partial^2 \cdot}{\partial y^2}$$

$L_1^*[v] = 0$ yields

$$\frac{\partial(yv)}{\partial y} + D_0 \frac{\partial^2 v}{\partial y^2} = 0$$

$$\implies \frac{y}{D_0} v + \frac{\partial v}{\partial y} = d_1$$

$$\implies \exp\left(\frac{y^2}{2D_0}\right) \frac{y}{D_0} v + \exp\left(\frac{y^2}{2D_0}\right) \frac{\partial v}{\partial y} = d_1 \exp\left(\frac{y^2}{2D_0}\right)$$

$$\implies \frac{\partial}{\partial y} \left[\exp\left(\frac{y^2}{2D_0}\right) v \right] = d_1 \exp\left(\frac{y^2}{2D_0}\right)$$

$$\implies \exp\left(\frac{y^2}{2D_0}\right) v(y) = d_1 \int_0^y \exp\left(\frac{z^2}{2D_0}\right) dz + d_0$$

$$\implies v(y) = d_1 \underbrace{\exp\left(\frac{-y^2}{2D_0}\right) \int_0^y \exp\left(\frac{z^2}{2D_0}\right) dz}_{\text{Not decaying to zero rapidly as } y \rightarrow \infty} + d_0 \exp\left(\frac{-y^2}{2D_0}\right)$$

Anyway, we select $v(y) = d_0 \exp\left(\frac{-y^2}{2D_0}\right)$

Step B5: Back to solvability of $L_1[u_2] = \frac{\partial u_0}{\partial t} + L_2[u_1]$.

We set d_0 to make $v(y)$ a normal density.

$$v(y) = \frac{1}{\sqrt{2\pi D_0}} \exp\left(\frac{-y^2}{2D_0}\right) = \rho_{N(0, D_0)}(y)$$

$$u_2 \text{ is solvable if and only if } \int_{-\infty}^{+\infty} \left(\frac{\partial u_0}{\partial t} + L_2[u_1] \right) \rho_{N(0, D_0)}(y) dy = 0.$$

Notice that $\partial u_0 / \partial t$ is independent of y . The solvability condition gives us

$$\frac{\partial u_0}{\partial t} + \int_{-\infty}^{+\infty} L_2[u_1] \rho_{N(0,D_0)}(y) dy = 0 \quad (\text{Cond-1})$$

Step B6: Calculation of $\int_{-\infty}^{+\infty} L_2[u_1] \rho_{N(0,D_0)}(y) dy$

Recall that $u_1 = y \frac{\partial u_0}{\partial x} + c_2(x, t) + c_3(x, t) \int_0^y \exp\left(\frac{z^2}{2D_0}\right) dz$. We calculate $L_2[u_1]$.

$$\begin{aligned} L_2[u_1] = & -y \frac{\partial u_1}{\partial x} - f(x, t) \frac{\partial u_1}{\partial y} = \underbrace{-y^2 \frac{\partial^2 u_0}{\partial x^2} - f(x, t) \frac{\partial u_0}{\partial x}}_{\text{effect of } u_0} - \underbrace{y \frac{\partial c_2}{\partial x}}_{\text{effect of } c_2} \\ & - \underbrace{y \frac{\partial c_3}{\partial x} \int_0^y \exp\left(\frac{z^2}{2D_0}\right) dz - f(x, t) c_3 \exp\left(\frac{y^2}{2D_0}\right)}_{\text{effect of } c_3} \end{aligned}$$

We examine the inner product of each part with $\rho_{N(0,D)}(y)$.

$u_0(x, t)$ is independent of y .

$$\int_{-\infty}^{+\infty} \underbrace{\left[-y^2 \frac{\partial^2 u_0}{\partial x^2} - f(x, t) \frac{\partial u_0}{\partial x} \right]}_{\text{effect of } u_0} \rho_{N(0,D_0)}(y) dy = -D_0 \frac{\partial^2 u_0}{\partial x^2} - f(x, t) \frac{\partial u_0}{\partial x}$$

$c_2(x, t)$ is independent of y .

$$\int_{-\infty}^{+\infty} \underbrace{-y \frac{\partial c_2}{\partial x}}_{\text{effect of } c_2} \rho_{N(0,D_0)}(y) dy = 0$$

$c_3(x, t)$ is independent of y .

$$\int_{-\infty}^{+\infty} \underbrace{\left[-y \frac{\partial c_3}{\partial x} \int_0^y \exp\left(\frac{z^2}{2D_0}\right) dz - f(x, t) c_3 \exp\left(\frac{y^2}{2D_0}\right) \right]}_{\text{effect of } c_3} \rho_{N(0,D_0)}(y) dy = \infty \quad \text{if } c_3 \neq 0.$$

To make $\int_{-\infty}^{+\infty} L_2[u_1] \rho_{N(0,D_0)}(y) dy$ finite, we must have $c_3(x, t) \equiv 0$.

Thus, we obtain the expression

$$\int_{-\infty}^{+\infty} L_2[u_1] \rho_{N(0,D_0)}(y) dy = -D_0 \frac{\partial^2 u_0}{\partial x^2} - f(x, t) \frac{\partial u_0}{\partial x} \quad (\text{Res-1})$$

Step B7: Governing equation for u_0

Substitute result (Res-1) into solvability condition (Cond-1), we conclude

$$\frac{\partial u_0}{\partial t} = D_0 \frac{\partial^2 u_0}{\partial x^2} + f(x, t) \frac{\partial u_0}{\partial x}$$

which is backward equation (BE-2).

Remark:

In the derivation above, the key is the method of solvability condition.

Below we illustrate the method of solvability condition in two simple examples.

Example: (the method of solvability condition)

Consider solving a 2×2 linear system $Ax = b$ where

$$A = \begin{pmatrix} 1 & 1+\varepsilon \\ 1+\varepsilon & 1 \end{pmatrix}, \quad b = \begin{pmatrix} 1-\varepsilon \\ 1+\varepsilon \end{pmatrix}$$

The exact solution is

$$x_{\text{exa}} = \begin{pmatrix} \frac{3+\varepsilon}{2+\varepsilon} \\ \frac{-(1+\varepsilon)}{2+\varepsilon} \end{pmatrix} \approx \begin{pmatrix} 1.5 \\ -0.5 \end{pmatrix}$$

Here we use asymptotic analysis to solve this example.

The goal is to see the application of solvability condition in a simple setting.

We seek solutions of the form

$$x = x^{(0)} + \varepsilon x^{(1)} + \dots$$

We write matrix A and vector b as

$$A = A^{(0)} + \varepsilon A^{(1)}, \quad A^{(0)} = \begin{pmatrix} 1 & 1 \\ 1 & 1 \end{pmatrix}, \quad A^{(1)} = \begin{pmatrix} 0 & 1 \\ 1 & 0 \end{pmatrix}$$

$$b = b^{(0)} + \varepsilon b^{(1)}, \quad b^{(0)} = \begin{pmatrix} 1 \\ 1 \end{pmatrix}, \quad b^{(1)} = \begin{pmatrix} -1 \\ 1 \end{pmatrix}$$

We expand linear system $Ax - b = 0$ into $O(1)$ terms, $O(\varepsilon)$ terms, ...

$$(A^{(0)} + \varepsilon A^{(1)})(x^{(0)} + \varepsilon x^{(1)} + \dots) - (b^{(0)} + \varepsilon b^{(1)}) = 0$$

$$\implies \left(A^{(0)}x^{(0)} - b^{(0)} \right) + \varepsilon \left(A^{(0)}x^{(1)} + A^{(1)}x^{(0)} - b^{(1)} \right) + \dots = 0$$

First we look at the $O(1)$ terms.

$$A^{(0)}x^{(0)} = b^{(0)}$$

This linear system is underdetermined.

$$\begin{pmatrix} 1 & 1 \\ 1 & 1 \end{pmatrix} \begin{pmatrix} x_1^{(0)} \\ x_2^{(0)} \end{pmatrix} = \begin{pmatrix} 1 \\ 1 \end{pmatrix}$$

$$\implies x_1^{(0)} + x_2^{(0)} = 1 \quad (\text{CNS-1})$$

From the $O(1)$ terms, we obtain only one constraint for two unknowns.

Next we look at the $O(\varepsilon)$ terms.

$$A^{(0)}x^{(1)} = -A^{(1)}x^{(0)} + b^{(1)} \quad (\text{L-1})$$

Matrix $A^{(0)}$ is symmetric. The null space of $A^{(0)}$ is

$$\text{Nul}(A^{(0)}) = \{v_0\}, \quad v_0 = \begin{pmatrix} 1 \\ -1 \end{pmatrix}$$

Linear system (L-1) is solvable if and only if

$$\langle -A^{(1)}x^{(0)} + b^{(1)}, v_0 \rangle = 0$$

$$\implies x_1^{(0)} - x_2^{(0)} - 2 = 0 \quad (\text{CNS-2})$$

Combining constraints (CNS-1) and (CNS-2), we conclude

$$x^{(0)} = \begin{pmatrix} 1.5 \\ -0.5 \end{pmatrix}$$

Example: (the method of solvability condition)

Consider the BVP of 2nd order linear ODE

$$\begin{cases} L[u] + \varepsilon x u = 3\sin(2x), & L[u] \equiv u'' + u \\ u(0) = 0, & u(\pi) = 0 \end{cases}$$

Here we use asymptotic analysis to solve this example.

We seek solutions of the form

$$u(x) = u^{(0)}(x) + \varepsilon u^{(1)}(x) + \dots$$

We expand the ODE into $O(1)$ terms, $O(\varepsilon)$ terms, ...

$$L[u^{(0)''}(x) + \varepsilon u^{(1)''}(x)] + \varepsilon x u^{(0)}(x) - 3\sin(2x) = 0$$

$$\implies \left(L[u^{(0)}(x)] - 3\sin(2x) \right) + \varepsilon \left(L[u^{(1)}(x)] + x u^{(0)}(x) \right) + \dots = 0$$

First we look at the $O(1)$ terms.

$$\begin{cases} L[u^{(0)}] = 3\sin(2x) \\ u^{(0)}(0) = 0, \quad u^{(0)}(\pi) = 0 \end{cases}$$

This BVP is underdetermined.

$$u^{(0)} = -\sin(2x) + c \sin(x) \quad \text{is a solution for any } c. \quad (\text{CNS-3})$$

Next we look at the $O(\varepsilon)$ terms.

$$\begin{cases} L[u^{(1)}] = -x u^{(0)}(x) \\ u^{(1)}(0) = 0, \quad u^{(1)}(\pi) = 0 \end{cases} \quad (\text{BVP-1})$$

Operator L with zero-BCs is self-adjoint (symmetric).

The null space of L with zero-BCs is

$$\text{Nul}(L) = \{v_0(x)\}, \quad v_0(x) = \sin(x)$$

(BVP-1) is solvable if and only if

$$\langle -x u^{(0)}(x), v_0 \rangle = 0$$

$$\implies \int_0^\pi (x \sin(2x) - c x \sin(x)) \sin(x) dx = 0$$

$$\implies -\frac{8}{9} - c \frac{\pi^2}{4} = 0 \quad \implies \quad c = \frac{-32}{9\pi^2} \quad (\text{CNS-4})$$

Combining constraints (CNS-3) and (CNS-4), we conclude

$$u^{(0)} = -\sin(2x) - \frac{32}{9\pi^2} \sin(x)$$